src/program_proof/simplepb/config_protocol_proof.v
@@ -67,8 +67,7 @@ Notation compute_reply := (Sm.compute_reply pb_record).
 Context `{!heapGS Σ}.
 Context `{!pbG Σ}.
 
-Definition is_Clerk2 ck γ : iProp Σ :=
-  ∃ γconf,
+Definition is_Clerk2 ck γ γconf : iProp Σ :=
     "#Hinv" ∷ is_conf_inv γ γconf ∗
     "#Hck" ∷ config_proof.is_Clerk ck γconf.
 
@@ -78,7 +77,7 @@ Lemma wp_MakeClerk2 (configHost:u64) γ :
   }}}
     config.MakeClerk #configHost
   {{{
-      ck, RET #ck; is_Clerk2 ck γ
+      γconf ck, RET #ck; is_Clerk2 ck γ γconf
   }}}.
 Proof.
   iIntros (Φ) "#Hhost HΦ".
@@ -86,11 +85,11 @@ Proof.
   wp_apply (config_proof.wp_MakeClerk with "[$Hhost]").
   iIntros.
   iApply "HΦ".
-  iExists  _; iFrame "#".
+  iFrame "#".
 Qed.
 
-Lemma wp_Clerk__GetConfig2 ck γ Φ :
-  is_Clerk2 ck γ -∗
+Lemma wp_Clerk__GetConfig2 ck γ γconf Φ :
+  is_Clerk2 ck γ γconf -∗
   □(∀ confγs (conf:list u64) config_sl,
   (is_slice_small config_sl uint64T 1 conf ∗
   ([∗ list] γsrv ; host ∈ confγs ; conf, is_pb_host host γ γsrv) -∗
@@ -125,10 +124,11 @@ Proof.
   iFrame "∗#".
 Qed.
 
-Lemma wp_Clerk__GetEpochAndConfig2 ck γ Φ :
-  is_Clerk2 ck γ -∗
+Lemma wp_Clerk_ReserveEpochAndConfig2 ck γ γconf Φ :
+  is_Clerk2 ck γ γconf -∗
   □((∀ (epoch epoch_lb:u64) confγs (conf:list u64) config_sl,
   (is_slice_small config_sl uint64T 1 conf ∗
+  is_reserved_epoch_lb γconf epoch ∗
   config_proposal_unset γ.(s_pb) epoch ∗
   own_proposal_unused γ.(s_pb) epoch ∗
   own_init_proposal_unused γ.(s_prim) epoch ∗
@@ -138,12 +138,12 @@ Lemma wp_Clerk__GetEpochAndConfig2 ck γ Φ :
   (∀ γsrv, ⌜γsrv ∈ (r_pb <$> confγs)⌝ → is_epoch_lb γsrv epoch_lb)) -∗
    Φ (#epoch, slice_val config_sl)%V
   )) -∗
-  WP config.Clerk__GetEpochAndConfig #ck {{ Φ }}
+  WP config.Clerk__ReserveEpochAndGetConfig #ck {{ Φ }}
 .
 Proof.
   iIntros "#Hck #HΦ".
   iNamed "Hck".
-  wp_apply (wp_Clerk__GetEpochAndConfig with "[$Hck]").
+  wp_apply (wp_Clerk__ReserveEpochAndGetConfig with "[$Hck]").
   iModIntro.
   iIntros "Hlc".
   iInv "Hinv" as "Hi" "Hclose".
@@ -154,11 +154,12 @@ Proof.
   iNamed "Hi".
   iExists _, _.
   iFrame.
-  iIntros "%Hno_overflow Hepoch Hconf".
+  iIntros "%Hno_overflow Hres Hconf".
+  iDestruct (mono_nat_lb_own_get with "Hres") as "#Hwit".
   iMod "Hmask".
 
   (* Hunset becomes skipped, and the first unused becomes unset. *)
-  iDestruct (big_sepS_elem_of_acc_impl (word.add epoch (U64 1)) with "Hunused") as "[Hunset_new Hunused]".
+  iDestruct (big_sepS_elem_of_acc_impl (word.add reservedEpoch (U64 1)) with "Hunreserved") as "[Hunset_new Hunused]".
   { set_solver. }
 
   iSpecialize ("Hunset_new" with "[]").
@@ -174,10 +175,10 @@ Proof.
     }
     iDestruct "Hskip1" as "#Hskip1".
 
-    iMod ("Hclose" with "[Hunset_new2 Hunused Hepoch Hconf]").
+    iMod ("Hclose" with "[Hres Hunset_new2 Hunused Hepoch Hconf]").
     {
       iNext. iExists _, _, _, _.
-      iFrame "Hepoch Hconf His_conf ∗#".
+      iFrame "Hepoch Hres Hconf His_conf ∗#".
       iSplitL "Hunused".
       {
         iApply "Hunused".
@@ -193,11 +194,11 @@ Proof.
         }
       }
       iIntros (???).
-      assert (int.nat epoch_skip = int.nat epoch ∨ int.nat epoch_skip < int.nat epoch ∨ int.nat epoch_skip >= int.nat (word.add epoch (U64 1))) as Hineq.
+      assert (int.nat epoch_skip = int.nat reservedEpoch ∨ int.nat epoch_skip < int.nat reservedEpoch ∨ int.nat epoch_skip >= int.nat (word.add reservedEpoch (U64 1))) as Hineq.
       { word. }
       destruct Hineq as [Heq|[Hineq|Hineq]].
       {
-        replace (epoch_skip) with (epoch) by word.
+        replace (epoch_skip) with (reservedEpoch) by word.
         iFrame "Hskip1".
       }
       {
@@ -215,11 +216,11 @@ Proof.
 
     (* TODO: repetetive proof *)
     iIntros.
-    assert (int.nat epoch_skip = int.nat epoch ∨ int.nat epoch_skip < int.nat epoch ∨ int.nat epoch_skip >= int.nat (word.add epoch (U64 1))) as Hineq.
+    assert (int.nat epoch_skip = int.nat reservedEpoch ∨ int.nat epoch_skip < int.nat reservedEpoch ∨ int.nat epoch_skip >= int.nat (word.add reservedEpoch (U64 1))) as Hineq.
     { word. }
     destruct Hineq as [Heq|[Hineq|Hineq]].
     {
-      replace (epoch_skip) with (epoch) by word.
+      replace (epoch_skip) with (reservedEpoch) by word.
       iFrame "Hskip1".
     }
     {
@@ -232,7 +233,7 @@ Proof.
   {
     iClear "His_skip".
 
-    iMod ("Hclose" with "[Hunset_new2 Hunused Hepoch Hconf]").
+    iMod ("Hclose" with "[Hres Hunset_new2 Hunused Hepoch Hconf]").
     {
       iNext. iExists _, _, _, _.
       iFrame "∗ His_conf #".
@@ -253,7 +254,7 @@ Proof.
       iIntros (???).
       exfalso.
       rewrite Hset in H.
-      replace (int.nat (word.add epoch 1%Z)) with (int.nat epoch + 1) in H0 by word.
+      replace (int.nat (word.add reservedEpoch 1%Z)) with (int.nat reservedEpoch + 1) in H0 by word.
       word.
     }
     iModIntro.
@@ -264,15 +265,16 @@ Proof.
     iIntros (???).
     exfalso.
     rewrite Hset in H.
-    replace (int.nat (word.add epoch 1%Z)) with (int.nat epoch + 1) in H0 by word.
+    replace (int.nat (word.add reservedEpoch 1%Z)) with (int.nat reservedEpoch + 1) in H0 by word.
     word.
   }
 Qed.
 
-Lemma wp_Clerk__WriteConfig2 ck γ Φ config_sl conf confγ epoch :
-  is_Clerk2 ck γ -∗
+Lemma wp_Clerk__WriteConfig2 ck γ γconf Φ config_sl conf confγ epoch :
+  is_Clerk2 ck γ γconf -∗
   is_slice_small config_sl uint64T 1 conf -∗
   is_epoch_config_proposal γ.(s_pb) epoch (r_pb <$> confγ) -∗
+  is_reserved_epoch_lb γconf epoch -∗
   ([∗ list] γsrv ; host ∈ confγ ; conf, is_pb_host host γ γsrv) -∗
   (∀ γsrv, ⌜γsrv ∈ (r_pb <$> confγ)⌝ → is_epoch_lb γsrv epoch) -∗
   □ (∀ (err:u64),
@@ -283,12 +285,12 @@ Lemma wp_Clerk__WriteConfig2 ck γ Φ config_sl conf confγ epoch :
       is_slice_small config_sl uint64T 1 conf -∗
       Φ #err)
   -∗
-  WP config.Clerk__WriteConfig #ck #epoch (slice_val config_sl) {{ Φ }}
+  WP config.Clerk__TryWriteConfig #ck #epoch (slice_val config_sl) {{ Φ }}
 .
 Proof.
-  iIntros "#Hck Hsl #Hconf_prop #Hhosts #Hlbs #HΦ".
+  iIntros "#Hck Hsl #Hconf_prop #Hwit #Hhosts #Hlbs #HΦ".
   iNamed "Hck".
-  wp_apply (wp_Clerk__WriteConfig with "Hck Hsl"); last first.
+  wp_apply (wp_Clerk__TryWriteConfig with "Hck Hsl"); last first.
   {
     iIntros.
     iApply ("HΦ" with "[] [$]").
@@ -296,6 +298,7 @@ Proof.
     { exfalso. done. }
     done.
   }
+  2:{ iFrame "#". }
   iModIntro.
   iIntros "Hlc".
   iInv "Hinv" as "Hi" "Hclose".
@@ -307,13 +310,13 @@ Proof.
   }
   iIntros "Hmask".
   iNamed "Hi".
-  iExists _.
+  iExists _, _.
   iFrame "∗".
   destruct (decide (_)); last first.
   { (* write failed because of stale epoch. *)
-    iIntros "Hepoch".
+    iIntros "Hepoch Hres".
     iMod "Hmask" as "_".
-    iMod ("Hclose" with "[Hepoch Hconf Hunused Hunset_or_set]").
+    iMod ("Hclose" with "[Hepoch Hres Hconf Hunreserved Hunset_or_set]").
     {
       iNext.  iExists _, _, _, _.
       iFrame "∗ His_conf #".
@@ -330,12 +333,12 @@ Proof.
     rewrite e.
     iExists _.
     iFrame.
-    iIntros "Hconf Hepoch".
+    iIntros "Hconf Hres Hepoch".
     iMod "Hmask" as "_".
 
     iDestruct "Hunset_or_set" as "[Hunset|%Hset]"; last first.
     { (* config was already set before *)
-      replace (epoch) with (epoch_lb) by word.
+      replace (epoch) with (epoch0) by word.
       iDestruct "Hconf_prop" as "[Hconf_prop %Hle]".
       iDestruct "His_conf" as "(? & His_conf_prop & ?)".
       iDestruct (own_valid_2 with "His_conf_prop Hconf_prop") as %Hvalid.
@@ -344,7 +347,7 @@ Proof.
       rewrite dfrac_agree_op_valid in Hvalid.
       replace (r_pb <$> confγs) with (r_pb <$> confγ) in * by naive_solver.
 
-      iMod ("Hclose" with "[Hepoch Hconf Hunused]").
+      iMod ("Hclose" with "[Hepoch Hconf Hunreserved Hres]").
       {
         iNext.  iExists _, _, _, _.
         iFrame "Hhosts ∗#".
@@ -365,7 +368,7 @@ Proof.
       iMod (own_update with "Hset") as "Hset".
       { apply singleton_update. apply dfrac_agree_persist. }
       iDestruct "Hset" as "#Hset".
-      iMod ("Hclose" with "[Hconf Hepoch Hunused]").
+      iMod ("Hclose" with "[Hconf Hres Hepoch Hunreserved]").
       {
         iNext. iExists _, _, _, _.
         iFrame "∗ Hset #".
